More cleanup

sepcomp/extspec.v
@@ -6,25 +6,35 @@ Require Import ListSet.
 
 (** External function specifications and linking *)
 
-Structure external_specification {M E Z:Type} := { 
-  ext_spec_type: E -> Type;
-  ext_spec_pre: forall e: E, 
-    ext_spec_type e -> list typ -> list val -> Z -> M -> Prop;
-  ext_spec_post: forall e: E, 
-    ext_spec_type e -> option typ -> option val -> Z -> M ->  Prop;
-  ext_spec_exit: option val -> Z -> M ->  Prop
-}.
-Implicit Arguments external_specification [].
+Structure external_specification (M E Z : Type) := 
+  { ext_spec_type : E -> Type
+  ; ext_spec_pre: forall e: E, 
+    ext_spec_type e -> list typ -> list val -> Z -> M -> Prop
+  ; ext_spec_post: forall e: E, 
+    ext_spec_type e -> option typ -> option val -> Z -> M ->  Prop
+  ; ext_spec_exit: option val -> Z -> M ->  Prop }.
+
+Arguments ext_spec_type {M E Z} _ _.
+Arguments ext_spec_pre {M E Z} _ _ _ _ _ _ _.
+Arguments ext_spec_post {M E Z} _ _ _ _ _ _ _.
+Arguments ext_spec_exit {M E Z} _ _ _ _.
 
 Definition ext_spec := external_specification mem external_function.
 
-Lemma extfunct_eqdec : forall ef1 ef2: external_function, {ef1=ef2} + {~ef1=ef2}.
-Proof. intros ef1 ef2; repeat decide equality; 
-  try apply Integers.Int.eq_dec.
+Lemma extfunct_eqdec (ef1 ef2 : external_function) : {ef1=ef2} + {~ef1=ef2}.
+Proof. 
+repeat decide equality; try apply Integers.Int.eq_dec.
 apply Floats.Float.eq_dec.
 Defined.
 
 Set Implicit Arguments.
+
+Definition ef_ext_spec (M Z : Type) := 
+  external_specification M AST.external_function Z.
+
+Definition spec_of 
+  (M Z : Type) (ef : AST.external_function) (spec : ef_ext_spec M Z) :=
+  (ext_spec_pre spec ef, ext_spec_post spec ef).
 
 Definition oval_inject j (v tv : option val) :=
   match v, tv with
@@ -33,7 +43,18 @@ Definition oval_inject j (v tv : option val) :=
     | _, _ => False
   end.
 
-Record injection_closed (Z : Type) (spec : ext_spec Z) :=
+Module ExtSpecProperties.
+
+Definition det (M E Z : Type) (spec : external_specification M E Z) :=
+  forall ef (x x' : ext_spec_type spec ef) tys z vals m
+         oty' ov' z' m' oty'' ov'' z'' m'',
+  ext_spec_pre spec ef x tys vals z m -> 
+  ext_spec_post spec ef x oty' ov' z' m' ->  
+  ext_spec_pre spec ef x' tys vals z m -> 
+  ext_spec_post spec ef x' oty'' ov'' z'' m'' ->  
+  oty'=oty'' /\ ov'=ov'' /\ z'=z'' /\ m'=m''.
+
+Record closed (Z : Type) (spec : ext_spec Z) :=
   { P_closed : 
       forall ef (x : ext_spec_type spec ef) j tys vals z m tvals tm, 
       ext_spec_pre spec ef x tys vals z m -> 
@@ -53,57 +74,6 @@ Record injection_closed (Z : Type) (spec : ext_spec Z) :=
       Mem.inject j m tm -> 
       ext_spec_exit spec otv z tm }.
 
-Definition ef_ext_spec (M Z: Type) := external_specification M AST.external_function Z.
+End ExtSpecProperties.
 
-Definition spec_of (M Z: Type) (ef: AST.external_function) (Sigma: ef_ext_spec M Z) :=
-  (ext_spec_pre Sigma ef, ext_spec_post Sigma ef).
-
-Section LinkExtSpec.
-Notation IN := (ListSet.set_mem extfunct_eqdec).
-Notation NOTIN := (fun ef l => ListSet.set_mem extfunct_eqdec ef l = false).
-Notation DIFF := (ListSet.set_diff extfunct_eqdec).
-
-Lemma in_diff (ef: AST.external_function) (l r: list AST.external_function): 
- IN ef l=true -> NOTIN ef r -> IN ef (DIFF l r)=true.
-Proof.
-simpl; intros H1 H2; apply set_mem_correct2. 
-apply set_mem_correct1 in H1.
-apply set_mem_complete1 in H2.
-apply set_diff_intro; auto.
-Qed.
-
-(** Linking external specification [Sigma] with an extension implementing
-   functions in [handled] *)
-
-Definition link_ext_spec (M Z: Type) (handled: AST.external_function -> Prop) 
-  (Sigma: external_specification M AST.external_function Z) :=
-  Build_external_specification M AST.external_function Z
-    (ext_spec_type Sigma)
-    (fun (ef: AST.external_function) (x: ext_spec_type Sigma ef)
-         (tys: list typ) (args: list val) (z: Z) (m: M) => 
-             ~handled ef /\ ext_spec_pre Sigma ef x tys args z m)
-    (fun (ef: AST.external_function) (x: ext_spec_type Sigma ef)
-         (ty: option typ) (ret: option val) (z: Z) (m: M) => 
-             handled ef \/ ext_spec_post Sigma ef x ty ret z m)
-    (ext_spec_exit Sigma).
-
-(** A client signature is linkable with an extension signature when each
-   extension function specification ef:{P}{Q} is a subtype of the
-   specification ef:{P'}{Q'} assumed by client. *)
-
-Definition linkable (M Z Zext: Type) (proj_zext: Z -> Zext)
-      (handled: AST.external_function -> Prop) 
-      (csig: ef_ext_spec M Z) (ext_sig: ef_ext_spec M Zext) := 
-  (forall ef P Q P' Q', 
-    ~handled ef -> 
-    spec_of ef ext_sig = (P, Q) -> 
-    spec_of ef csig = (P', Q') -> 
-    forall x' tys args m z, P' x' tys args z m -> 
-      exists x, P x tys args (proj_zext z) m /\
-      forall ty ret m' z', Q x ty ret (proj_zext z') m' -> Q' x' ty ret z' m') /\
-  (forall ret z m,
-    ext_spec_exit ext_sig ret (proj_zext z) m -> 
-    ext_spec_exit csig ret z m).
-
-End LinkExtSpec.
 
